src/BBCommon.v
@@ -1,0 +1,281 @@
+
+From Coq Require Import List ZArith.
+From mathcomp Require Import ssreflect ssrnat ssrbool eqtype seq tuple.
+From BitBlasting Require Import Var QFBV CNF.
+From ssrlib Require Import SsrOrdered Tactics.
+
+Set Implicit Arguments.
+Unset Strict Implicit.
+Import Prenex Implicits.
+
+Definition cnf_lit_not a := [:: [:: neg_lit a]].
+Definition cnf_lit_xor a1 a2 := [:: [:: a1; a2]; [:: neg_lit a1; neg_lit a2]].
+Definition cnf_lit_eq a1 a2 := [:: [:: neg_lit a1; a2]; [:: a1; neg_lit a2]].
+
+Lemma cnf_lit_not_negb E b l :
+  enc_bit E l b -> (interp_cnf E (cnf_lit_not l)) = (~~ b).
+Proof.
+  rewrite /enc_bit /cnf_lit_not /=. rewrite interp_lit_neg_lit. by move/eqP => ->.
+Qed.
+
+Lemma cnf_lit_xor_neqb E b1 b2 l1 l2 :
+  enc_bit E l1 b1 -> enc_bit E l2 b2 ->
+  (interp_cnf E (cnf_lit_xor l1 l2)) = (b1 != b2).
+Proof.
+  rewrite /enc_bit /cnf_lit_xor /=. rewrite !interp_lit_neg_lit.
+  move=> /eqP -> /eqP ->. by case: b1; case: b2.
+Qed.
+
+Lemma cnf_lit_eq_eqb E b1 b2 l1 l2 :
+  enc_bit E l1 b1 -> enc_bit E l2 b2 ->
+  (interp_cnf E (cnf_lit_eq l1 l2)) = (b1 == b2).
+Proof.
+  rewrite /enc_bit /cnf_lit_eq /=. rewrite !interp_lit_neg_lit.
+  move=> /eqP -> /eqP ->. by case: b1; case: b2.
+Qed.
+
+
+
+(* ===== Variable generation ===== *)
+
+Definition generator := positive.
+
+Definition gen (g : generator) : generator * literal := (g + 1, Pos g)%positive.
+
+
+
+(* ===== A map from variables to literal representation ===== *)
+
+Definition vm := VM.t word.
+
+
+
+(* ===== newer_than_vm ===== *)
+
+Definition newer_than_vm g (m : vm) :=
+  forall v rs, VM.find v m = Some rs -> newer_than_lits g rs.
+
+Lemma newer_than_vm_add_r x m y : newer_than_vm x m -> newer_than_vm (x + y) m.
+Proof.
+  move=> Hnew v rs Hfind. move: (Hnew v rs Hfind). exact: newer_than_lits_add_r.
+Qed.
+
+Lemma newer_than_vm_le_newer x m y :
+  newer_than_vm x m -> (x <=? y)%positive -> newer_than_vm y m.
+Proof.
+  move=> Hnew Hle v rs Hfind. move: (Hnew v rs Hfind) => {Hnew} Hnew.
+  exact: (newer_than_lits_le_newer Hnew Hle).
+Qed.
+
+
+
+(* ===== Consistent ===== *)
+
+Definition consistent1 m E s v : Prop :=
+    match VM.find v m with
+    | None => True
+    | Some rs => enc_bits E rs (QFBV.State.acc v s)
+    end.
+Definition consistent m E s := forall v, consistent1 m E s v.
+
+Lemma consistent_env_upd_newer m s E g g' b :
+  newer_than_vm g m -> consistent m E s -> (g <=? g')%positive ->
+  consistent m (env_upd E g' b) s.
+Proof.
+  move=> Hnew Hcon Hle. move: (newer_than_vm_le_newer Hnew Hle) => Hnew'. move=> v.
+  move: (Hnew' v) (Hcon v) => {Hnew Hnew' Hcon}. rewrite /consistent1.
+  case: (VM.find v m); last by done. move=> rs Hnew Henc.
+  move: (Hnew rs (Logic.eq_refl (Some rs))) => {Hnew} Hnew.
+  rewrite (newer_than_lits_enc_bits_env_upd _ _ _ Hnew). exact: Henc.
+Qed.
+
+Lemma env_preserve_consistent m E E' g s :
+  newer_than_vm g m -> env_preserve E E' g -> consistent m E s -> consistent m E' s.
+Proof.
+  move=> Hnew_gm Hpre Hcon. move=> x; rewrite /consistent1.
+  case Hfind: (VM.find x m); last by done. move: (Hnew_gm x _ Hfind) => Hnew_glsx.
+  move: (Hcon x); rewrite /consistent1. rewrite Hfind.
+  exact: (env_preserve_enc_bits Hpre Hnew_glsx).
+Qed.
+
+
+
+(* ===== vm_preserve ===== *)
+
+Definition vm_preserve (m m' : vm) : Prop :=
+  forall v ls, VM.find v m = Some ls -> VM.find v m' = Some ls.
+
+Lemma vm_preserve_consistent m m' s E :
+  vm_preserve m m' -> consistent m' E s -> consistent m E s.
+Proof.
+  move=> Hpre Hcon v. rewrite /consistent1. case Hfind: (VM.find v m) => //=.
+  move: (Hpre _ _ Hfind) => Hfind'. move: (Hcon v). rewrite /consistent1.
+  rewrite Hfind'. by apply.
+Qed.
+
+Lemma vm_preserve_refl m : vm_preserve m m.
+Proof. done. Qed.
+
+Lemma vm_preserve_trans m1 m2 m3 :
+  vm_preserve m1 m2 -> vm_preserve m2 m3 -> vm_preserve m1 m3.
+Proof. move=> H12 H23 v ls Hfind1. apply: H23. apply: H12. assumption. Qed.
+
+Lemma vm_preserve_add_diag m v ls :
+  VM.find v m = None -> vm_preserve m (VM.add v ls m).
+Proof.
+  move=> Hfind x xls Hfindx. case Hxv: (x == v).
+  - rewrite (eqP Hxv) Hfind in Hfindx. discriminate.
+  - move/negP: Hxv => Hxv. rewrite (VM.Lemmas.find_add_neq _ _ Hxv). assumption.
+Qed.
+
+
+
+(* ===== Tactics ===== *)
+
+Ltac fresh_name t :=
+  match t with
+  | vm => fresh "m"
+  | env => fresh "E"
+  | generator => fresh "g"
+  | cnf => fresh "cs"
+  | _.-tuple literal => fresh "ls"
+  | literal => fresh "l"
+  | _ => fresh
+  end.
+
+Ltac dcase_hyps :=
+  match goal with
+  | H : context f [let '_ := ?r in _] |- _ =>
+    move: H;
+    let H1 := fresh in
+    let H2 := fresh in
+    lazymatch type of r with
+    | prod (prod (prod (prod ?t1 ?t2) ?t3) ?t4) ?t5 =>
+      let t1 := fresh_name t1 in
+      let t2 := fresh_name t2 in
+      let t3 := fresh_name t3 in
+      let t4 := fresh_name t4 in
+      let t5 := fresh_name t5 in
+      dcase r; move=> [[[[t1 t2] t3] t4] t5] H1 H2; dcase_hyps
+    | prod (prod (prod ?t1 ?t2) ?t3) ?t4 =>
+      let t1 := fresh_name t1 in
+      let t2 := fresh_name t2 in
+      let t3 := fresh_name t3 in
+      let t4 := fresh_name t4 in
+      dcase r; move=> [[[t1 t2] t3] t4] H1 H2; dcase_hyps
+    | prod (prod ?t1 ?t2) ?t3 =>
+      let t1 := fresh_name t1 in
+      let t2 := fresh_name t2 in
+      let t3 := fresh_name t3 in
+      dcase r; move=> [[t1 t2] t3] H1 H2; dcase_hyps
+    | prod ?t1 ?t2 =>
+      let t1 := fresh_name t1 in
+      let t2 := fresh_name t2 in
+      dcase r; move=> [t1 t2] H1 H2; dcase_hyps
+    end
+  | H : context f [if ?c then _ else _] |- _ =>
+    move: H;
+    let H1 := fresh in
+    let H2 := fresh in
+    dcase c=> H1 H2; dcase_hyps
+  | H : (_, _, _, _, _) = (_, _, _, _, _) |- _ =>
+    case: H;
+    let H1 := fresh in
+    let H2 := fresh in
+    let H3 := fresh in
+    let H4 := fresh in
+    let H5 := fresh in
+    move=> H1 H2 H3 H4 H5; dcase_hyps
+  | H : (_, _, _, _) = (_, _, _, _) |- _ =>
+    case: H;
+    let H1 := fresh in
+    let H2 := fresh in
+    let H3 := fresh in
+    let H4 := fresh in
+    move=> H1 H2 H3 H4; dcase_hyps
+  | H : (_, _, _) = (_, _, _) |- _ =>
+    case: H;
+    let H1 := fresh in
+    let H2 := fresh in
+    let H3 := fresh in
+    move=> H1 H2 H3; dcase_hyps
+  | H : (_, _) = (_, _) |- _ =>
+    case: H;
+    let H1 := fresh in
+    let H2 := fresh in
+    move=> H1 H2; dcase_hyps
+  | H : context f [match ?t with | None => _ | Some _ => _ end] |- _ =>
+    move: H;
+    let H1 := fresh in
+    let H2 := fresh in
+    dcase t; case => H1 H2; dcase_hyps
+  | H : context f [match ?t with | Some _ => _ | None => _ end] |- _ =>
+    move: H;
+    let H1 := fresh in
+    let H2 := fresh in
+    dcase t; case => H1 H2; dcase_hyps
+  | |- _ => idtac
+  end.
+
+Ltac dcase_goal :=
+  match goal with
+  | |- context f [let '_ := ?r in _] =>
+    let H := fresh in
+    lazymatch type of r with
+    | prod (prod (prod (prod ?t1 ?t2) ?t3) ?t4) ?t5 =>
+      let t1 := fresh_name t1 in
+      let t2 := fresh_name t2 in
+      let t3 := fresh_name t3 in
+      let t4 := fresh_name t4 in
+      let t5 := fresh_name t5 in
+      dcase r; move=> [[[[t1 t2] t3] t4] t5] H; dcase_goal
+    | prod (prod (prod ?t1 ?t2) ?t3) ?t4 =>
+      let t1 := fresh_name t1 in
+      let t2 := fresh_name t2 in
+      let t3 := fresh_name t3 in
+      let t4 := fresh_name t4 in
+      dcase r; move=> [[[t1 t2] t3] t4] H; dcase_goal
+    | prod (prod ?t1 ?t2) ?t3 =>
+      let t1 := fresh_name t1 in
+      let t2 := fresh_name t2 in
+      let t3 := fresh_name t3 in
+      dcase r; move=> [[t1 t2] t3] H; dcase_goal
+    | prod ?t1 ?t2 =>
+      let t1 := fresh_name t1 in
+      let t2 := fresh_name t2 in
+      dcase r; move=> [t1 t2] H; dcase_goal
+    end
+  | |- (_, _, _, _, _) = (_, _, _, _, _) =>
+    let H1 := fresh in
+    let H2 := fresh in
+    let H3 := fresh in
+    let H4 := fresh in
+    let H5 := fresh in
+    case=> H1 H2 H3 H4 H5; dcase_goal
+  | |- (_, _, _, _) = (_, _, _, _) =>
+    let H1 := fresh in
+    let H2 := fresh in
+    let H3 := fresh in
+    let H4 := fresh in
+    case=> H1 H2 H3 H4; dcase_goal
+  | |- (_, _, _) = (_, _, _) =>
+    let H1 := fresh in
+    let H2 := fresh in
+    let H3 := fresh in
+    case=> H1 H2 H3; dcase_goal
+  | |- (_, _) = (_, _) =>
+    let H1 := fresh in
+    let H2 := fresh in
+    case=> H1 H2; dcase_goal
+  | |- _ => idtac
+  end.
+
+Ltac dite_hyps :=
+  match goal with
+  | H : context f [if ?c then _ else _] |- _ =>
+    move: H;
+    let H1 := fresh in
+    let H2 := fresh in
+    dcase c; case=> H1 H2; dite_hyps
+  | |- _ => idtac
+  end.
