src/BBVar.v
@@ -1,0 +1,156 @@
+
+From Coq Require Import ZArith List.
+From mathcomp Require Import ssreflect ssrbool ssrnat eqtype seq.
+From BitBlasting Require Import Var QFBV CNF BBCommon.
+From ssrlib Require Import ZAriths Tactics.
+From nbits Require Import NBits.
+
+Set Implicit Arguments.
+Unset Strict Implicit.
+Import Prenex Implicits.
+
+
+
+(* ===== bit_blast_var ===== *)
+
+Fixpoint bit_blast_var' (g : generator) (w : nat) : generator * word :=
+  match w with
+  | O => (g, [::])
+  | S n => let (g', hd) := gen g in
+           let (g'', tl) := bit_blast_var' g' n in
+           (g'', hd::tl)
+  end.
+
+Fixpoint mk_env_var' E g bs : env * generator * word :=
+  match bs with
+  | [::] => (E, g, [::])
+  | bs_hd::bs_tl => let (g', hd) := gen g in
+                    let E' := env_upd E (var_of_lit hd) bs_hd in
+                    let '(E'', g'', tl) := mk_env_var' E' g' bs_tl in
+                    (E'', g'', hd::tl)
+  end.
+
+Definition bit_blast_var g (v : var) : generator * cnf * word :=
+  let (g', vs) := bit_blast_var' g (vsize v) in
+  (g', [::], vs).
+
+Definition mk_env_var E g (bs : bits) (v : var) : env * generator * cnf * word :=
+  let '(E', g', vs) := mk_env_var' E g bs in
+  (E', g', [::], vs).
+
+Lemma bit_blast_var_cnf_empty g v g' cs lrs :
+  bit_blast_var g v = (g', cs, lrs) -> cs = [::].
+Proof.
+  rewrite /bit_blast_var. dcase (bit_blast_var' g (vsize v)).
+  move=> [g_v lrs_v] Hbb. by case=> _ <- _.
+Qed.
+
+Lemma mk_env_var'_is_bit_blast_var' E g bs E' g' lrs :
+  mk_env_var' E g bs = (E', g', lrs) -> bit_blast_var' g (size bs) = (g', lrs).
+Proof.
+  elim: bs g E E' g' lrs => [|bs_hd bs_tl IH] /=.
+  - by move=> ? ? ? ? ? [] _ <- <-.
+  - move=> ig iE oE og olrs.
+    dcase (mk_env_var' (env_upd iE ig bs_hd) (ig+1)%positive bs_tl).
+    move=> [[E g] lrs] Henv. case=> _ <- <-. by rewrite (IH _ _ _ _ _ Henv).
+Qed.
+
+Lemma mk_env_var_is_bit_blast_var E g bs v E' g' cs lrs :
+  size bs = vsize v -> mk_env_var E g bs v = (E', g', cs, lrs) ->
+  bit_blast_var g v = (g', cs, lrs).
+Proof.
+  rewrite /mk_env_var /bit_blast_var. dcase (mk_env_var' E g bs).
+  move=> [[E_env g_env] ls_env] Henv <-. rewrite (mk_env_var'_is_bit_blast_var' Henv).
+  by case=> _ <- <- <-.
+Qed.
+
+Lemma mk_env_var_sat E g bs v E' g' cs lrs :
+  size bs = vsize v -> mk_env_var E g bs v = (E', g', cs, lrs) ->
+  interp_cnf E' cs.
+Proof.
+  rewrite /mk_env_var => Hs. dcase (mk_env_var' E g bs) => [[[oE og] olrs] Henv].
+  by case=> <- _ <- _.
+Qed.
+
+Lemma mk_env_var'_preserve E g bs E' g' lrs :
+  mk_env_var' E g bs = (E', g', lrs) -> env_preserve E E' g.
+Proof.
+  elim: bs E g E' g' lrs => [| bs_hd bs_tl IH] /=.
+  - move=> ? ? ? ? ? [] <- _ _. exact: env_preserve_refl.
+  - move=> E g E' g' lrs.
+    dcase (mk_env_var' (env_upd E g bs_hd) (g + 1)%positive bs_tl).
+    move=> [[oE og] olrs] Henv. case=> <- _ _. move: (IH _ _ _ _ _ Henv).
+    exact: env_preserve_env_upd_succ.
+Qed.
+
+Lemma mk_env_var_preserve E g bs v E' g' cs lrs :
+  mk_env_var E g bs v = (E', g', cs, lrs) -> env_preserve E E' g.
+Proof.
+  rewrite /mk_env_var. dcase (mk_env_var' E g bs) => [[[oE og] olrs] Henv].
+  case=> <- _ _ _. exact: (mk_env_var'_preserve Henv).
+Qed.
+
+Lemma mk_env_var'_newer_gen E g bs E' g' lrs :
+  mk_env_var' E g bs = (E', g', lrs) -> (g <=? g')%positive.
+Proof.
+  elim: bs E g E' g' lrs => [| bs_hd bs_tl IH] /=.
+  - move=> ? ? ? ? ? [] _ <- _. exact: Pos.leb_refl.
+  - move=> E g E' g' lrs.
+    dcase (mk_env_var' (env_upd E g bs_hd) (g + 1)%positive bs_tl).
+    move=> [[oE og] olrs] Henv. case=> _ <- _. move: (IH _ _ _ _ _ Henv).
+    apply: pos_leb_trans. exact: pos_leb_add_diag_r.
+Qed.
+
+Lemma mk_env_var_newer_gen E g bs v E' g' cs lrs :
+  mk_env_var E g bs v = (E', g', cs, lrs) -> (g <=? g')%positive.
+Proof.
+  rewrite /mk_env_var. dcase (mk_env_var' E g bs) => [[[oE og] olrs] Henv].
+  case=> _ <- _ _. exact: (mk_env_var'_newer_gen Henv).
+Qed.
+
+Lemma mk_env_var'_newer_res E g bs E' g' lrs :
+  mk_env_var' E g bs = (E', g', lrs) -> newer_than_lits g' lrs.
+Proof.
+  elim: bs E g E' g' lrs => [| bs_hd bs_tl IH] /=.
+  - by move=> ? ? ? ? ? [] _ <- <-.
+  - move=> E g E' g' lrs.
+    dcase (mk_env_var' (env_upd E g bs_hd) (g + 1)%positive bs_tl).
+    move=> [[oE og] olrs] Henv. case=> _ <- <-. rewrite newer_than_lits_cons.
+    rewrite (IH _ _ _ _ _ Henv) andbT. rewrite /newer_than_lit /newer_than_var /=.
+    move: (mk_env_var'_newer_gen Henv) => H. apply: (pos_ltb_leb_trans _ H).
+    exact: pos_ltb_add_diag_r.
+Qed.
+
+Lemma mk_env_var_newer_res E g bs v E' g' cs lrs :
+  mk_env_var E g bs v = (E', g', cs, lrs) -> newer_than_lits g' lrs.
+Proof.
+  rewrite /mk_env_var. dcase (mk_env_var' E g bs) => [[[oE og] olrs] Henv].
+  case=> _ <- _ <-. exact: (mk_env_var'_newer_res Henv).
+Qed.
+
+Lemma mk_env_var_newer_cnf E g bs v E' g' cs lrs :
+  mk_env_var E g bs v = (E', g', cs, lrs) -> newer_than_cnf g' cs.
+Proof.
+  rewrite /mk_env_var. dcase (mk_env_var' E g bs) => [[[oE og] olrs] Henv].
+  by case=> _ <- <- _.
+Qed.
+
+Lemma mk_env_var'_enc E g bs E' g' lrs :
+  mk_env_var' E g bs = (E', g', lrs) -> enc_bits E' lrs bs.
+Proof.
+  elim: bs E g E' g' lrs => [| bs_hd bs_tl IH] //=.
+  - by move=> ? ? ? ? ? [] <- _ <-.
+  - move=> E g E' g' lrs.
+    dcase (mk_env_var' (env_upd E g bs_hd) (g + 1)%positive bs_tl).
+    move=> [[oE og] olrs] Henv. case=> <- _ <-. rewrite enc_bits_cons.
+    rewrite (IH _ _ _ _ _ Henv) andbT. move: (mk_env_var'_preserve Henv) => Hpre.
+    apply: (env_preserve_enc_bit Hpre (newer_than_lit_add_diag_r (Pos g) 1)).
+    exact: enc_bit_env_upd_eq_pos.
+Qed.
+
+Lemma mk_env_var_enc E g bs v E' g' cs lrs :
+  mk_env_var E g bs v = (E', g', cs, lrs) -> enc_bits E' lrs bs.
+Proof.
+  rewrite /mk_env_var. dcase (mk_env_var' E g bs) => [[[oE og] olrs] Henv].
+  case=> <- _ _ <-. exact: (mk_env_var'_enc Henv).
+Qed.
